

# Durrett 5th Chapter1 Solutions

htao

November 11, 2025

## 1 Probability Spaces

**1.1.1.** Let  $\Omega = \mathbb{R}$ ,  $\mathcal{F}$  = all subsets so that  $A$  or  $A^c$  is countable,  $P(A) = 0$  in the first case and  $= 1$  in the second. Show that  $(\Omega, \mathcal{F}, P)$  is a probability space.

**Solution.** We firstly prove  $\mathcal{F}$  is a  $\sigma$ -field. Let  $\{A_i\} \subseteq \mathcal{F}$ . It is obvious  $A_i^c \in \mathcal{F}$ . If  $A_i$  or  $A_j$  is countable, then  $A_i \cap A_j$  is countable and hence contained in  $\mathcal{F}$ . Otherwise  $A_i^c$  and  $A_j^c$  is countable, and then  $(A_i \cap A_j)^c = A_i^c \cup A_j^c$  is countable, which concludes  $A_i \cap A_j$  is always in  $\mathcal{F}$ . Finally,  $\bigcup_{i \in \mathbb{N}} A_i$  is countable if every  $A_i$  is countable, Otherwise  $(\bigcup_{i \in \mathbb{N}} A_i)^c = \bigcap_{i \in \mathbb{N}} A_i^c \subseteq A_0^c$  is countable since  $A_0^c$  is countable, which concludes  $\bigcup_{i \in \mathbb{N}} A_i \in \mathcal{F}$ . Hence  $\mathcal{F}$  is a  $\sigma$ -field.

$P$  is well-defined since  $A \cup A^c = \Omega = \mathbb{R}$  is uncountable, whence  $A$  and  $A^c$  can not be countable simultaneously. Finally we prove  $P$  is a probability. It is trivial  $P(\Omega) = 1$ . For disjoint sets,  $A_i \in \mathcal{F}$ , if  $A_i$  are all countable,  $P(A_i) = 0$  and then  $\bigcup_{i=1}^{\infty} A_i$  is countable,  $P(\bigcup_{i=1}^{\infty} A_i) = 0 = \sum_{i=1}^{\infty} P(A_i)$ . Otherwise  $A_k^c$  is countable, and then  $A_i \subseteq A_k^c, i \neq k$  is countable since they are disjoint. And  $(\bigcup_{i \in \mathbb{N}} A_i)^c = \bigcap_{i \in \mathbb{N}} A_i^c \subseteq A_k^c$  is countable. So  $P(\bigcup_{i=1}^{\infty} A_i) = \sum_{i=1}^{\infty} P(A_i) = 1 = P(\bigcup_{i \in \mathbb{N}} A_i)$ , when  $P$  is a probability.  $\square$

**1.1.2.** Recall the definition of  $S_d$  from Example 1.1.5. Show that  $\sigma(S_d) = \mathcal{R}^d$ , the Borel subsets of  $\mathbb{R}^d$ .

*Proof.* The definition of  $S_d$  is

$$S_d = \left\{ \prod_{i=1}^d (a_i, b_i] \mid -\infty \leq a, b \leq +\infty \right\}$$

It is obvious  $S_d \subseteq \mathcal{R}^d$  whence  $\sigma(S_d) \subseteq \mathcal{R}^d$ . Then for any  $\prod_{i=1}^d (a_i, b_i)$ ,

$$\bigcup_{n=1}^{\infty} \left( \prod_{i=1}^d (a_i, b_i - \frac{1}{n}] \right) = \prod_{i=1}^d (a_i, b_i)$$

The desired result follows from  $\mathcal{R}^d$  is the  $\sigma$ -field of the right.

**1.1.3.** A  $\sigma$ -field  $\mathcal{F}$  is said to be countably generated if there is a countable collection  $\mathcal{C} \subseteq \mathcal{F}$  so that  $\sigma(\mathcal{C}) = \mathcal{F}$ . Show that  $\mathcal{R}^d$  is countably generated.

**Solution.** Let

$$\mathcal{U} = \left\{ \prod_{i=1}^d (a_i, b_i) \mid a_i, b_i \in \mathbb{Q} \right\}$$

Then  $\mathcal{U}$  is countable since  $|\mathcal{U}| \leq |\mathbb{Q}^{2d}|$ . And  $\sigma(\mathcal{U}) = \mathcal{R}^d$  since for each  $\prod_{i=1}^d (a_i, b_i)$ , there are  $a_{i,k}, b_{i,k} \in \mathbb{Q}$  such that  $a_{i,k} \rightarrow a_i + 0$  and  $b_{i,k} \rightarrow b_i - 0$  as  $k \rightarrow \infty$  and then

$$\bigcup_{k=1}^{\infty} \left( \prod_{i=1}^d (a_{i,k}, b_{i,k}) \right) = \prod_{i=1}^d (a_i, b_i)$$

$\square$

#### 1.1.4.

- (i) Show that if  $\mathcal{F}_1 \subseteq \mathcal{F}_2 \subseteq \dots$  are  $\sigma$ -algebras, then  $\bigcup_i \mathcal{F}_i$  is an algebra.  
(ii) Give an example to show that  $\bigcup_i \mathcal{F}_i$  need not be a  $\sigma$ -algebra.

**Solution.**

- (i) For  $A, B \in \bigcup_i \mathcal{F}_i$ , there is  $F_k$  such that  $A, B \in \mathcal{F}_k$ , and then  $A \cup B, A^c \in \mathcal{F}_k \subseteq \bigcup_i \mathcal{F}_i$ , whence  $\bigcup_i \mathcal{F}_i$  is an algebra.  
(ii) Let  $\Omega = \mathbb{R}^{\mathbb{N}}$  and  $F_i = \{U \times \mathbb{R}^{\mathbb{N}} \mid U \in \mathcal{R}^i\}$ . While  $[0, 1]^i \times \mathbb{R}^{\mathbb{N}} \in \mathcal{F}_i$ , but

$$[0, 1]^{\mathbb{N}} = \bigcap_{i=1}^{\infty} [0, 1]^i \times \mathbb{R}^{\mathbb{N}} \notin \bigcup_i \mathcal{F}_i$$

□

**1.1.5.** A set  $A \subseteq \{1, 2, \dots\}$  is said to have asymptotic density  $\theta$  if

$$\lim_{n \rightarrow \infty} \frac{|A \cap \{1, 2, \dots, n\}|}{n} = \theta$$

Let  $\mathcal{A}$  be the collection of sets for which the asymptotic density exists. Is  $\mathcal{A}$  a  $\sigma$ -algebra? an algebra?

**Solution.**  $\mathcal{A}$  is not an algebra. The counterexample is shown in the following.

Let  $A = \{2n\}$  and  $B = \{b_n\}, b_n \in \{2n-1, 2n\}$ . Then  $A, B$  have asymptotic densities  $1/2$ . And then let

$$S_n = |A \cap B \cap \{1, 2, \dots, 2n\}| = \sum_{k=1}^n |A \cap B \cap \{2k-1, 2k\}| = \sum_{k=1}^n c_k$$

where

$$c_k = \begin{cases} 0 & b_k = 2k-1 \\ 1 & b_k = 2k \end{cases}$$

It means for any series  $\{x_i\}, x_i \in \{0, 1\}$ , there exists  $B$  with asymptotic density  $1/2$  such that  $c_i = x_i$ . Hence let

$$c_i = \begin{cases} 0 & i = 1 \\ 1 & i = [3^{2k} + 1, 3^{2k+1}] \\ 0 & i = [3^{2k+1} + 1, 3^{2k+2}] \end{cases} \quad k \in \mathbb{N}$$

Then for  $n = 3^{2k+1}$ ,  $S_n \geq \sum_{3^{2k+1}}^{3^{2k+1}} c_i = 2 \times 3^{2k} = \frac{2}{3}n$  and for  $n = 3^{2k+2}$ ,  $S_n = S_{3^{2k+1}} \leq 3^{2k+1} = \frac{1}{3}n$ . So  $L_n := |A \cap B \cap \{1, 2, \dots, n\}|/n \geq 1/3$  when  $n = 2 \times 3^{2k+1}$  and  $L_n \leq \frac{1}{6}$  when  $n = 2 \times 3^{2k+2}$ , whence  $L_n$  diverges and then  $\mathcal{A}$  is not an algebra.

(The motivation here is for  $0 < S_n/n < 1$  we could add a lot of 1's to making  $S_{n+m}/n+m > 1-\epsilon$  for any epsilon; and a lot of 0's to making  $S_{n+m}/n+m < \epsilon$  for any  $\epsilon > 0$ . Thus the quotient could fluctuates and then not converge.) □

## 2 Distributions

**1.2.1.** Suppose  $X$  and  $Y$  are random variables on  $(\Omega, \mathcal{F}, P)$  and let  $A \in \mathcal{F}$ . Show that if we let  $Z(\omega) = X(\omega)$  for  $\omega \in A$  and  $Z(\omega) = Y(\omega)$  for  $\omega \in A^c$ , then  $Z$  is a random variable.

**Solution.**  $Z = X \cdot 1_A + Y \cdot 1_{A^c}$  is a random variable. □

**1.2.2.** Let  $\chi$  have the standard normal distribution. Use Theorem 1.2.6 to get upper and lower bounds on  $P(\chi \leq 4)$ .

**Solution.** Theorem 1.2.6 is listed at Theorem 1.2.2.

$$P(\chi \leq 4) = \int_{-\infty}^4 e^{x^2/2} dx = 1 - \int_x^{+\infty} e^{x^2/2} dx$$

Applying the theorem gives

$$\left(\frac{1}{4} - \frac{1}{64}\right)e^{-8} \leq \int_x^{+\infty} e^{x^2/2} dx \leq \frac{1}{4}e^{-8}$$

So

$$1 - \frac{1}{4}e^{-8} \leq P(\chi \leq 4) \leq 1 - \frac{15e^{-8}}{64}$$

□

**1.2.3.** Show that a distribution function has at most countably many discontinuities.

**Solution.** This is a common conclusion in real analysis. Let  $f$  be a distribution function, then  $f$  is monotonic increasing. Let  $P$  be the set of discontinuities. For each  $x_0 \in P$ ,  $f_-(x_0)$ ,  $f_+(x_0)$  exist and  $f_-(x_0) < f_+(x_0)$ . Then letting

$$\mathcal{I} := \{(f_-(a), f_+(a)) \mid a \in P\}$$

and

$$\begin{aligned} \varphi : P &\rightarrow \mathcal{I} \\ x_0 &\mapsto (f_-(x_0), f_+(x_0)) \end{aligned}$$

intervals in  $\mathcal{I}$  are disjoint and  $\varphi$  is bijective and in since for any  $x < y$ ,

$$f_-(x) < f_+(x) \leq f_-(y) < f_+(y)$$

The desired result follows from  $\mathcal{I}$ , a collection of disjoint open intervals in  $\mathbb{R}$ , is at most countable since  $\exists q_{a,b} \in \mathbb{Q}$ ,  $q_{a,b} \in (a,b) \in \mathcal{I}$ , and then  $(a,b) \mapsto q_{a,b}$  is an injection to  $\mathbb{Q}$ . □

**1.2.4.** Show that if  $F(x) = P(X \leq x)$  is continuous then  $Y = F(X)$  has a uniform distribution on  $(0, 1)$ , that is, if  $y \in [0, 1]$ ,  $P(Y \leq y) = y$ .

*Proof.* We have  $0 \leq F(x) \leq 1$ , so  $P(Y \leq y) = 0$  for  $y < 0$  and  $P(Y \leq y) = 1$  for  $y > 1$ . For  $y \in [0, 1]$ ,

$$P(Y \leq y) = P(F(X) \leq y) = P(X \in \{h \mid F(h) \leq y\})$$

Let  $h_0 = \sup \{h \mid F(h) \leq y\}$ . Since  $F$  is increasing and continuous,  $F(h_0) = y$ . Therefore

$$P(Y \leq y) = P(X \leq h_0) = F(h_0) = y$$

**1.2.5.** Suppose  $X$  has continuous density  $f$ ,  $P(\alpha \leq X \leq \beta) = 1$  and  $g$  is a function that is strictly increasing and differentiable on  $(\alpha, \beta)$ . Then  $g(X)$  has density

$$\rho(y) = \begin{cases} \frac{f(g^{-1}(y))}{g'(g^{-1}(y))} & y \in (g(\alpha), g(\beta)) \\ 0 & \text{otherwise} \end{cases}$$

When  $g(x) = ax + b$  with  $a > 0$ ,  $g^{-1}(y) = \frac{y-b}{a}$  so the answer is  $\frac{1}{a}f(\frac{y-b}{a})$ .

*Proof.* Since  $g$  is strictly increasing,  $g$  is invertible and therefore

$$P(g(X) \leq y) = P(X \leq g^{-1}(y)) = \begin{cases} 0 & y \in (-\infty, g(\alpha)] \\ \int_{\alpha}^{g^{-1}(y)} f(x) dx & y \in (g(\alpha), g(\beta)) \\ 1 & y \in [g(\beta), +\infty) \end{cases}$$

We could direct differentiate the right or replace  $x = g^{-1}(u)$ , and then

$$\int_{\alpha}^{g^{-1}(y)} f(x) dx = \int_{g(\alpha)}^y f(g^{-1}(u)) dg^{-1}(u) = \int_{g(\alpha)}^y \frac{f(g^{-1}(u))}{g'(g^{-1}(u))} du$$

**1.2.6.** Suppose  $X$  has a normal distribution. Use the previous exercise to compute the density of  $\exp(X)$ . (The answer is called the lognormal distribution.)

*Proof.* By Exercise 1.2.5, letting  $f(x) = \frac{1}{\sqrt{2\pi}} e^{-x^2/2}$ , the distribution is

$$g(x) = \begin{cases} \frac{f(\ln x)}{\exp(\ln(x))} = \frac{1}{x\sqrt{2\pi}} e^{-\frac{(\ln x)^2}{2}} & x \in (0, +\infty) \\ 0 & x \in (-\infty, 0] \end{cases}$$

**1.2.7.**

- (i) Suppose  $X$  has density function  $f$ . Compute the distribution function of  $X^2$  and then differentiate to find its density function.
- (ii) Work out the answer when  $X$  has a standard normal distribution to find the density of the chi-square distribution.

*Proof.*

- (i) Since

$$P(X^2 \leq y) = \begin{cases} 0 & y \in (-\infty, 0] \\ P(-\sqrt{y} \leq X \leq \sqrt{y}) & y \in (0, +\infty) \end{cases}$$

and replacing  $x = \sqrt{u}$ ,

$$\begin{aligned} P(-\sqrt{y} \leq X \leq \sqrt{y}) &= \int_{-\sqrt{y}}^{\sqrt{y}} f(x) dx = \int_0^{\sqrt{y}} (f(x) + f(-x)) dx \\ &= \int_0^y (f(\sqrt{u}) + f(-\sqrt{u})) d\sqrt{u} = \int_0^y \frac{f(\sqrt{u}) + f(-\sqrt{u})}{2\sqrt{u}} du \end{aligned}$$

$X^2$  has a density function,

$$g(y) = \begin{cases} 0 & y \in (-\infty, 0] \\ \frac{f(\sqrt{y}) + f(-\sqrt{y})}{2\sqrt{y}} & y \in (0, +\infty) \end{cases}$$

(We can not directly differentiate the definite integrals with variable limits, since it may be indifferentiable when  $f$  is discontinuous)

- (ii) Applying above conclusion, the density is

$$g(y) = \begin{cases} 0 & y \in (-\infty, 0] \\ \frac{e^{-y/2}}{\sqrt{2\pi y}} & y \in (0, +\infty) \end{cases}$$

## A Some related theorem details

### 2 Distributions

**Theorem 1.2.1.** For  $x > 0$ , letting

$$I(x) := \int_x^{+\infty} e^{-y^2/2}$$

then for  $n \in \mathbb{N}$ ,

$$I(x) = I_n(x) + R_n(x)$$

where

$$\begin{aligned} I_n(x) &:= e^{-x^2/2} \left( \frac{1}{x} - \frac{1}{x^3} + \frac{3}{x^5} - \frac{15}{x^7} + \cdots + (-1)^{n-1} \frac{(2n-3)!!}{x^{2n-1}} \right) \\ &= e^{-x^2/2} \sum_{k=1}^n (-1)^{k-1} \frac{(2k-3)!!}{x^{2k-1}} \end{aligned}$$

and

$$R_n(x) := (-1)^n (2n-1)!! \int_x^{+\infty} \frac{e^{-y^2/2}}{y^{2n}} dy$$

by setting  $(-1)!! = 1$ . Then  $I_{2k}(x) < I(x) < I_{2k+1}(x)$  for any  $k \in \mathbb{N}$ .

*Proof.* Use induction on  $n$ . It's trivial for  $n = 0$  and assume it holds for  $n = k$ . Since

$$\begin{aligned} \frac{R_k(x)}{(-1)^k (2k-1)!!} &= \int_x^\infty \frac{e^{-y^2/2}}{y^{2k}} dy = \int_x^{+\infty} -\frac{1}{y^{2k+1}} de^{-y^2/2} \\ &= \left. \frac{-e^{-y^2/2}}{y^{2k+1}} \right|_x^{+\infty} - \int_x^{+\infty} \frac{(2k+1)e^{-y^2/2}}{y^{2k+2}} dy \\ &= \frac{-e^{-x^2/2}}{x^{2k+1}} - (2k+1) \int_x^{+\infty} \frac{e^{-y^2/2}}{y^{2k+2}} dy \\ &= \frac{-e^{-x^2/2}}{x^{2k+1}} + \frac{R_{k+1}(x)}{(-1)^k (2k-1)!!} \end{aligned}$$

then

$$\begin{aligned} I &= I_k + R_k = I_k + (-1)^k (2k-1)!! \frac{-e^{-x^2/2}}{x^{2k+1}} + R_{k+1}(x) \\ &= I_{k+1}(x) + R_{k+1}(x) \end{aligned}$$

The last conclusion is obvious since  $R_{2k} > 0$  and  $R_{2k+1} < 0$  for any  $k \in \mathbb{N}$ .

*Proof.*

**Theorem 1.2.2** (Theorem 1.2.6 in PTE5th). *For  $x > 0$ ,*

$$(x^{-1} - x^{-3})e^{-x^2/2} \leq \int_x^{+\infty} e^{-y^2/2} dy \leq x^{-1}e^{-x^2/2}$$

*Proof.* We give a stronger conclusion and a more general proof in Theorem 1.2.1. The desired result directly follows from the cases of  $n = 1$  and  $n = 2$ .